Refactor by "params"

ConsensusSafety.thy
@@ -29,6 +29,30 @@ type_synonym state = "message set"
 (* NOTE: We parameterized estimator by weight. *)
 type_synonym estimator = "weight \<Rightarrow> state \<Rightarrow> consensus_value set"
 
+(* CBC Casper parameters *)
+datatype params = 
+  Params "validator set * weight * threshold * consensus_value set * estimator"
+
+fun V :: "params \<Rightarrow> validator set"
+  where
+    "V (Params (v_set, _, _, _, _)) = v_set"
+
+fun W :: "params \<Rightarrow> weight"
+  where
+    "W (Params (_, weight, _, _, _)) = weight"
+
+fun t :: "params \<Rightarrow> threshold"
+  where
+    "t (Params (_, _, threshold, _, _)) = threshold"
+
+fun C :: "params \<Rightarrow> consensus_value set"
+  where
+    "C (Params (_, _, _, c_set, _)) = c_set"
+
+fun \<epsilon> :: "params \<Rightarrow> estimator"
+  where
+    "\<epsilon> (Params (_, _, _, _, estimator)) = estimator"
+
 
 (* Section 2.2: Protocol Definition *)
 
@@ -43,77 +67,79 @@ fun est :: "message \<Rightarrow> consensus_value"
 
 fun justification :: "message \<Rightarrow> state"
   where
-    "justification (Message (_, _, ml)) = set ml"
+    "justification (Message (_, _, s)) = set s"
 
 (* Definition 2.7 *)
-fun is_valid :: "weight \<Rightarrow>(estimator \<Rightarrow> (message \<Rightarrow> bool))"
+definition is_valid :: "params \<Rightarrow> message \<Rightarrow> bool"
   where
-    "is_valid w e (Message (c, v, s)) = (c \<in> e w (set s))"
+    "is_valid params m = (est m \<in> \<epsilon> params (W params) (justification m))"
 
-(* FIXME: Can we construct valid_message type? Currently we assume all states are valid in all the 
-"definition"s and use is_valid_state for all occurrences of state type in lemmas. *)
-definition is_valid_state :: "weight \<Rightarrow> estimator \<Rightarrow> state \<Rightarrow> bool"
+(* NOTE: Currently we assume all state type variables are valid in all the 
+definitions and use `is_valid_state` for all occurrences of state type in lemmas and theorems. *)
+definition is_valid_state :: "params \<Rightarrow> state \<Rightarrow> bool"
   where
-    "is_valid_state w e s = (\<forall> m \<in> s. is_valid w e m)"
+    "is_valid_state params \<sigma> = (\<forall> m \<in> \<sigma>. is_valid params m)"
 
 (* Definition 2.8: Protocol state transitions \<rightarrow> *)
-definition is_future_state :: "state \<Rightarrow> state \<Rightarrow> bool"
+fun is_future_state :: "(state * state) \<Rightarrow> bool"
   where
-    "is_future_state s1 s2 = (s1 \<supseteq> s2)"
+    "is_future_state(\<sigma>1, \<sigma>2) = (\<sigma>1 \<supseteq> \<sigma>2)"
 
 (* Definition 2.9 *)
-definition equivocation :: "message \<Rightarrow> message \<Rightarrow> bool"
+fun equivocation :: "(message * message) \<Rightarrow> bool"
   where
-    "equivocation m1 m2 =
-      (sender m1 = sender m2 \<and> m1 \<noteq> m2 \<and> m1 \<notin> justification(m2) \<and> m2 \<notin> justification(m1))"
+    "equivocation(m1, m2) =
+      (sender m1 = sender m2 \<and> m1 \<noteq> m2 \<and> m1 \<notin> justification m2 \<and> m2 \<notin> justification m1)"
 
 (* Definition 2.10 *)
 definition equivocating_validators :: "state \<Rightarrow> validator set"
   where
-    "equivocating_validators s = 
-      {v. \<exists> m1 m2. m1 \<in> s \<and> m2 \<in> s \<and> equivocation m1 m2 \<and> sender m1 = v}"
+    "equivocating_validators \<sigma> = 
+      {v. \<exists> m1 m2. m1 \<in> \<sigma> \<and> m2 \<in> \<sigma> \<and> equivocation(m1, m2) \<and> sender m1 = v}"
 
 (* Definition 2.11 *)
-definition equivocation_fault_weight :: "weight \<Rightarrow> state \<Rightarrow> int"
+definition equivocation_fault_weight :: "params \<Rightarrow> state \<Rightarrow> int"
   where
-    "equivocation_fault_weight w s = sum w (equivocating_validators s)"
+    "equivocation_fault_weight params \<sigma> = sum (W params) (equivocating_validators \<sigma>)"
 
 (* Definition 2.12 *)
-definition is_faults_lt_threshold :: "threshold \<Rightarrow> weight \<Rightarrow> state \<Rightarrow> bool"
+definition is_faults_lt_threshold :: "params \<Rightarrow> state \<Rightarrow> bool"
   where 
-    "is_faults_lt_threshold t w s = (equivocation_fault_weight w s < t)"
+    "is_faults_lt_threshold params \<sigma> = (equivocation_fault_weight params \<sigma> < t params)"
+
 
 (* Section 3: Safety Proof *)
 (* Section 3.1: Guaranteeing Common Futures *)
 
 (* Definition 3.1 *)
-definition futures :: "threshold \<Rightarrow> weight \<Rightarrow> state \<Rightarrow> state set"
+definition futures :: "params \<Rightarrow> state \<Rightarrow> state set"
   where
-    "futures t w s = {s'. is_faults_lt_threshold t w s' \<and> is_future_state s' s}"
+    "futures params \<sigma> = {\<sigma>'. is_faults_lt_threshold params \<sigma>' \<and> is_future_state(\<sigma>', \<sigma>)}"
 
 (* Lemma 1 *)
 lemma monotonic_futures :
-  "\<forall> s' s. is_faults_lt_threshold t w s' \<and> is_faults_lt_threshold t w s
-   \<and> is_valid_state w e s' \<and> is_valid_state w e s
-   \<Longrightarrow> (s' \<in> futures t w s \<longleftrightarrow> futures t w s' \<subseteq> futures t w s)"
-   using futures_def is_future_state_def by auto
+  "\<forall> params \<sigma>' \<sigma>. is_faults_lt_threshold params \<sigma>' \<and> is_faults_lt_threshold params \<sigma>
+   \<and> is_valid_state params \<sigma>' \<and> is_valid_state params \<sigma>
+   \<Longrightarrow> (\<sigma>' \<in> futures params \<sigma> \<longleftrightarrow> futures params \<sigma>' \<subseteq> futures params \<sigma>)"
+   using futures_def by auto
 
 notation Set.empty ("\<emptyset> ")
 
 (* Theorem 1 *)
 theorem two_party_common_futures :
-  "\<forall> s1 s2. is_faults_lt_threshold t w s1 \<and> is_faults_lt_threshold t w s2
-   \<and> is_valid_state w e s1 \<and> is_valid_state w e s2
-  \<Longrightarrow> is_faults_lt_threshold t w (s1 \<union> s2)
-  \<Longrightarrow> futures t w s1 \<inter> futures t w s2 \<noteq> \<emptyset>"
-  using futures_def is_future_state_def by auto
+  "\<forall> params \<sigma>1 \<sigma>2. is_faults_lt_threshold params \<sigma>1 \<and> is_faults_lt_threshold params \<sigma>2
+   \<and> is_valid_state params \<sigma>1 \<and> is_valid_state params \<sigma>2
+  \<Longrightarrow> is_faults_lt_threshold params (\<sigma>1 \<union> \<sigma>2)
+  \<Longrightarrow> futures params \<sigma>1 \<inter> futures params \<sigma>2 \<noteq> \<emptyset>"
+  using futures_def  by auto
 
 (* Theorem 2 *)
 theorem n_party_common_futures :
-  "\<forall> s_set. \<forall> s. s \<in> s_set \<and> is_faults_lt_threshold t w s \<and> is_valid_state w e s
-  \<Longrightarrow> is_faults_lt_threshold t w (\<Union> s_set)
-  \<Longrightarrow> futures t w s1 \<inter> futures t w s2 \<noteq> \<emptyset>"
+  "\<forall> params \<sigma>_set. \<forall> \<sigma>. \<sigma> \<in> \<sigma>_set \<and> is_faults_lt_threshold params \<sigma> \<and> is_valid_state params s
+  \<Longrightarrow> is_faults_lt_threshold params (\<Union> \<sigma>_set)
+  \<Longrightarrow> futures params \<sigma>1 \<inter> futures params \<sigma>2 \<noteq> \<emptyset>"
   by blast
+
 
 (* Section 3.2: Guaranteeing Consistent Decisions *)
 (* Section 3.2.1: Guaranteeing Consistent Decisions on Properties of Protocol States *)
@@ -122,57 +148,56 @@ theorem n_party_common_futures :
 type_synonym state_property = "state \<Rightarrow> bool"
 
 (* Definition 3.3  *)
-definition state_property_is_decided :: "threshold \<Rightarrow> weight \<Rightarrow> state_property \<Rightarrow> state \<Rightarrow> bool"
+fun state_property_is_decided :: "params \<Rightarrow> (state_property * state) \<Rightarrow> bool"
   where
-    "state_property_is_decided t w p s = (\<forall> s'. s' \<in> futures t w s \<and> p s')"
+    "state_property_is_decided params (p, \<sigma>) = (\<forall> \<sigma>'. \<sigma>' \<in> futures params \<sigma> \<and> p \<sigma>')"
 
 (* Lemma 2 *)
 lemma forward_consistency :
-  "\<forall> s' s. is_faults_lt_threshold t w s' \<and> is_faults_lt_threshold t w s
-   \<and> is_valid_state w e s' \<and> is_valid_state w e s \<and> (\<forall> s'. s' \<in> futures t w s) 
-  \<Longrightarrow> state_property_is_decided t w p s
-  \<Longrightarrow> state_property_is_decided t w p s'"
-  by (simp add: state_property_is_decided_def)
+  "\<forall> params \<sigma>' \<sigma>. is_faults_lt_threshold params \<sigma>' \<and> is_faults_lt_threshold params \<sigma>
+   \<and> is_valid_state params \<sigma>' \<and> is_valid_state params \<sigma> \<and> (\<forall> \<sigma>'. \<sigma>' \<in> futures params \<sigma>) 
+  \<Longrightarrow> state_property_is_decided params (p, \<sigma>)
+  \<Longrightarrow> state_property_is_decided params (p, \<sigma>')"
+  by auto
 
 (* Lemma 3 *)
 lemma backword_consistency :
-  "\<forall> s' s. is_faults_lt_threshold t w s' \<and> is_faults_lt_threshold t w s
-   \<and> is_valid_state w e s' \<and> is_valid_state w e s \<and> (\<forall> s'. s' \<in> futures t w s) 
-  \<Longrightarrow> state_property_is_decided t w p s'
-  \<Longrightarrow> \<not>state_property_is_decided t w (\<lambda>s. (\<not> p s)) s"
-  by (simp add: state_property_is_decided_def)
+  "\<forall> params \<sigma>' \<sigma>. is_faults_lt_threshold params \<sigma>' \<and> is_faults_lt_threshold params \<sigma>
+   \<and> is_valid_state params \<sigma>' \<and> is_valid_state params \<sigma> \<and> (\<forall> \<sigma>'. \<sigma>' \<in> futures params \<sigma>)
+  \<Longrightarrow> state_property_is_decided params (p, \<sigma>')
+  \<Longrightarrow> \<not>state_property_is_decided params (\<lambda>\<sigma>''. (\<not> p \<sigma>''), \<sigma>)"
+  by auto
   
 (* Theorem 3 *)
 theorem two_party_consensus_safety :
-  "\<forall> s1 s2. is_faults_lt_threshold t w s1 \<and> is_faults_lt_threshold t w s2
-   \<and> is_valid_state w e s1 \<and> is_valid_state w e s2
-  \<Longrightarrow> is_faults_lt_threshold t w (s1 \<union> s2)
-  \<Longrightarrow> \<not>(state_property_is_decided t w p s1 \<and> state_property_is_decided t w (\<lambda>s. (\<not> p s)) s2)"
-  apply (simp add: state_property_is_decided_def)
-  by blast  
+  "\<forall> params \<sigma>1 \<sigma>2. is_faults_lt_threshold params \<sigma>1 \<and> is_faults_lt_threshold params \<sigma>2
+   \<and> is_valid_state params \<sigma>1 \<and> is_valid_state params \<sigma>2
+  \<Longrightarrow> is_faults_lt_threshold params (\<sigma>1 \<union> \<sigma>2)
+  \<Longrightarrow> \<not>(state_property_is_decided params (p, \<sigma>1) \<and> state_property_is_decided params (\<lambda>\<sigma>. (\<not> p \<sigma>), \<sigma>2))"
+  by auto
 
 (* Definition 3.4 *)
 (* NOTE: We can use \<And> to make it closer to the paper? *)
-definition state_properties_are_inconsistent :: "weight \<Rightarrow> estimator \<Rightarrow> state_property set \<Rightarrow> bool"
+definition state_properties_are_inconsistent :: "params \<Rightarrow> state_property set \<Rightarrow> bool"
   where
-    "state_properties_are_inconsistent w e p_set = (\<forall> s. is_valid_state w e s \<and> \<not> (\<forall> p. p \<in> p_set \<and> p s))"
+    "state_properties_are_inconsistent params p_set = (\<forall> \<sigma>. is_valid_state params \<sigma> \<and> \<not> (\<forall> p. p \<in> p_set \<and> p \<sigma>))"
 
 (* Definition 3.5 *)
-definition state_properties_are_consistent :: "weight \<Rightarrow> estimator \<Rightarrow> state_property set \<Rightarrow> bool"
+definition state_properties_are_consistent :: "params \<Rightarrow> state_property set \<Rightarrow> bool"
   where
-    "state_properties_are_consistent w e p_set = (\<exists> s. is_valid_state w e s \<and> (\<forall> p. p \<in> p_set \<and> p s))"
+    "state_properties_are_consistent params p_set = (\<exists> \<sigma>. is_valid_state params \<sigma> \<and> (\<forall> p. p \<in> p_set \<and> p \<sigma>))"
 
 (* Definition 3.6 *)
-definition state_property_decisions :: "threshold \<Rightarrow> weight \<Rightarrow> state \<Rightarrow> state_property set"
+definition state_property_decisions :: "params \<Rightarrow> state \<Rightarrow> state_property set"
   where 
-    "state_property_decisions t w s = {p. state_property_is_decided t w p s}"
+    "state_property_decisions params \<sigma> = {p. state_property_is_decided params (p, \<sigma>)}"
 
 (* Theorem 4 *)
 (* NOTE: We can use \<Union> to make it closer to the paper? *)
 theorem n_party_safety_for_state_properties :
-  "\<forall> s_set. \<forall> s. s \<in> s_set \<and> is_faults_lt_threshold t w s \<and> is_valid_state w e s
-  \<Longrightarrow> is_faults_lt_threshold t w (\<Union> s_set)
-  \<Longrightarrow> state_properties_are_consistent w e {p. \<exists> s. s \<in> s_set \<and> p \<in> state_property_decisions t w s}" 
+  "\<forall> params \<sigma>_set \<sigma>. \<sigma> \<in> \<sigma>_set \<and> is_faults_lt_threshold params \<sigma> \<and> is_valid_state params \<sigma>
+  \<Longrightarrow> is_faults_lt_threshold params (\<Union> \<sigma>_set)
+  \<Longrightarrow> state_properties_are_consistent params {p. \<exists> \<sigma>. \<sigma> \<in> \<sigma>_set \<and> p \<in> state_property_decisions params \<sigma>}" 
   by blast
 
 (* Section 3.2.2: Guaranteeing Consistent Decisions on Properties of Consensus Values *)
@@ -180,9 +205,9 @@ theorem n_party_safety_for_state_properties :
 type_synonym consensus_value_property = "consensus_value \<Rightarrow> bool"
 
 (* Definition 3.8 *)
-definition naturally_corresponding_state_property :: "weight \<Rightarrow> estimator \<Rightarrow> consensus_value_property \<Rightarrow> state_property"
+definition naturally_corresponding_state_property :: "params \<Rightarrow> consensus_value_property \<Rightarrow> state_property"
   where 
-    "naturally_corresponding_state_property w e p = (\<lambda>s. \<forall>c. c \<in> e w s \<and> p c)"
+    "naturally_corresponding_state_property params p = (\<lambda>\<sigma>. \<forall>c. c \<in> \<epsilon> params (W params) \<sigma> \<and> p c)"
 
 (* Definition 3.9 *)
 (* NOTE: Here the type of `c` is inferred correctly? *)
@@ -192,25 +217,25 @@ definition consensus_value_properties_are_consistent :: "consensus_value_propert
 
 (* Lemma 4 *)
 lemma naturally_corresponding_consistency :
-  "\<forall> p_set. state_properties_are_consistent w e {naturally_corresponding_state_property w e p | p. p \<in> p_set}
+  "\<forall> params p_set. state_properties_are_consistent params {naturally_corresponding_state_property params p | p. p \<in> p_set}
     \<Longrightarrow> consensus_value_properties_are_consistent p_set"
   using state_properties_are_consistent_def by auto
 
 (* Definition 3.10 *)
-definition consensus_value_property_is_decided :: "threshold \<Rightarrow> weight \<Rightarrow> estimator \<Rightarrow> consensus_value_property \<Rightarrow> state \<Rightarrow> bool"
+fun consensus_value_property_is_decided :: "params \<Rightarrow> (consensus_value_property * state) \<Rightarrow> bool"
   where
-    "consensus_value_property_is_decided t w e p s = state_property_is_decided t w (naturally_corresponding_state_property w e p) s "
+    "consensus_value_property_is_decided params (p, \<sigma>) = state_property_is_decided params ((naturally_corresponding_state_property params p), \<sigma>)"
 
 (* Definition 3.11 *)
-definition consensus_value_property_decisions :: "threshold \<Rightarrow> weight \<Rightarrow> estimator \<Rightarrow> state \<Rightarrow> consensus_value_property set"
+definition consensus_value_property_decisions :: "params \<Rightarrow> state \<Rightarrow> consensus_value_property set"
   where
-    "consensus_value_property_decisions t w e s = {p. consensus_value_property_is_decided t w e p s}"
+    "consensus_value_property_decisions params \<sigma> = {p. consensus_value_property_is_decided params (p, \<sigma>)}"
 
 (* Theorem 5 *)
 theorem n_party_safety_for_consensus_value_properties :
-  "\<forall> s_set. \<forall> s. s \<in> s_set \<and> is_faults_lt_threshold t w s \<and> is_valid_state w e s
-  \<Longrightarrow> is_faults_lt_threshold t w (\<Union> s_set)
-  \<Longrightarrow> consensus_value_properties_are_consistent {p. \<exists> s. s \<in> s_set \<and> p \<in> consensus_value_property_decisions t w e s}"
+  "\<forall> params \<sigma>_set. \<forall> \<sigma>. \<sigma> \<in> \<sigma>_set \<and> is_faults_lt_threshold params \<sigma> \<and> is_valid_state params \<sigma>
+  \<Longrightarrow> is_faults_lt_threshold params (\<Union> \<sigma>_set)
+  \<Longrightarrow> consensus_value_properties_are_consistent {p. \<exists> \<sigma>. \<sigma> \<in> \<sigma>_set \<and> p \<in> consensus_value_property_decisions params \<sigma>}"
   by blast
 
 end
